debruijn and normal term equality using lgterms defined

cbn_cem.v
@@ -1,10 +1,11 @@
 Require cem cbn expr db relations.
+Require Import Minus.
 Require Import Unicode.Utf8 List NaryFunctions.
 Require Import expr_db util CpdtTactics.
 Require Import Basics.
 Require Import Compare_dec.
 
-Definition fresh (e : list nat) (h : cem.heap):= maximum (e ++ domain h). 
+Open Scope program_scope. 
 
 (* We define a term type with local and global variables to allow us to have an
    equality relation between the cem and cbn configurations *)
@@ -42,37 +43,185 @@ Definition seq_option {a b} : option (a → b) → option a → option b := λ f
 Notation "f <$> x" := (fmap_option f x) (at level 30).
 Notation "f <*> x" := (seq_option f x) (at level 40).
 
+Fixpoint cte (t:db.tm) (d:nat) : lgexpr := match t with
+  | db.lam b => lam (cte b (S d))
+  | db.app m n => app (cte m d) (cte n d)
+  | db.var v => if gt_dec d v then lvar v else gvar (v-d)
+  end.
+
+Fixpoint fvs' (t:db.tm) (d:nat) : list nat := match t with
+  | db.lam b => fvs' b (S d)
+  | db.app m n => fvs' m d ++ fvs' n d
+  | db.var v => if gt_dec d v then nil else (v-d)::nil
+  end.
+
+Lemma filter_app {A} : ∀ xs ys (p:A → bool), filter p xs ++ filter p ys = filter p (xs ++ ys). 
+intros. induction xs. reflexivity. simpl. destruct (p a). simpl. 
+rewrite <- IHxs. reflexivity. apply IHxs. Qed. 
+
+Lemma fvs_eq : ∀ t d, map (λ x, x - d) (filter (λ x, if gt_dec d x then false
+else true) (db.fvs t)) = fvs' t d.
+intros t. induction t; intros. simpl. destruct (gt_dec d n). reflexivity. simpl.
+reflexivity. simpl. assert (∀ xs d, map (λ x : nat, x - S d) (filter (λ x : nat, if gt_dec
+(S d) x then false else true) xs) = map (λ x :
+nat, x - d) (filter (λ x : nat, if gt_dec d x then false else true) (map pred
+(remove 0 xs)))). intros. induction xs. reflexivity. destruct a. simpl. apply
+IHxs. simpl. destruct (gt_dec d0 a). apply Gt.gt_n_S in g. destruct (gt_dec (S
+d0) (S a)). apply IHxs. apply n in g. inversion g. destruct (gt_dec (S d0) (S
+a)). apply Gt.gt_S_n in g. apply n in g. inversion g. simpl. rewrite IHxs.
+reflexivity. specialize IHt with (S d). rewrite <- IHt. rewrite H. reflexivity.
+simpl. rewrite <- IHt1. rewrite <- IHt2. rewrite <- map_app. rewrite <-
+filter_app. reflexivity. Qed. 
+
+Lemma fvs_eq_zero : ∀ t, db.fvs t = fvs' t 0.
+intros. rewrite <- fvs_eq. simpl. induction (db.fvs t). simpl. reflexivity. 
+simpl. rewrite <- minus_n_O. rewrite <- IHl. reflexivity. Qed. 
+
+Fixpoint gfvs (t:lgexpr) : list nat := match t with
+  | lam b => gfvs b
+  | app m n => gfvs m ++ gfvs n
+  | gvar v => v::nil
+  | lvar v => nil
+  end.
+
+Lemma gfvs_fvs : ∀ t d, gfvs (cte t d) = fvs' t d.
+intros t. induction t; intros. simpl. destruct (gt_dec d n). reflexivity. reflexivity.
+apply IHt. simpl. rewrite IHt1. rewrite IHt2. reflexivity. Qed.
+
+Lemma forevery_in {A} : ∀ (x:A) xs p, In x xs → forevery xs p → p x.
+intros. induction xs. simpl in H. inversion H. simpl in H. destruct H. simpl in
+H0. subst. destruct H0. assumption. simpl in H0. destruct H0. specialize (IHxs H
+H1). assumption. Qed. 
+
+Lemma forevery_subset {A} : ∀ xs ys (p:A→Prop), xs ⊆ ys → forevery ys p → forevery xs p.
+intros. induction xs. auto. simpl. simpl in H. destruct H. apply IHxs in H1.
+split. apply (forevery_in _ _ _ H H0). assumption. Qed.
+
+Lemma cte_lu : ∀ t d v, cte t d = gvar (d-v) → In (d-v) (fvs' t d). 
+intros. destruct t; inversion H. simpl. destruct (gt_dec d n). inversion H1. inversion
+H1. rewrite H2. simpl. apply (or_introl eq_refl). Qed. 
+
 (* Converting a debruijn term requires a full configuration, we don't change
    local variables, and traverse the cactus stack to find the final location of the
    closure corresponding to a variable and a cactus location *)
-Definition conftolg : cem.configuration → option lgexpr := λ c, match c with 
-  | cem.conf h (cem.close t e) => let fix cte t dep :=
+Definition conftolg (c: cem.configuration) (d:nat): option lgexpr := match c with
+  | cem.conf h (cem.close t e) => let t' := cte t d in let fix cte' t :=
     match t with
-    | db.lam b => lam <$> cte b (S dep)
-    | db.app m n => app <$> cte m dep <*> cte n dep
-    | db.var v => if gt_dec dep v 
-      then Some (lvar v)
-      else (λ x, gvar (fst x)) <$> cem.clu (dep - v) e h
-    end in cte t 0
+    | lam b => lam <$> (cte' b) 
+    | app m n => app <$> (cte' m) <*> (cte' n)
+    | lvar v => Some (lvar v)
+    | gvar v => (gvar ∘ @fst nat _) <$> cem.clu v e h
+    end in cte' t'  
   end.
+
+Lemma clu_some_lu : ∀ v e h x, cem.clu v e h = Some x → ∃ y, lookup e h = Some y.
+intros. unfold cem.clu in H. remember (lookup e h). destruct o. exists c.
+reflexivity. induction v. rewrite <- Heqo in H. inversion H. rewrite <- Heqo in
+H. inversion H. Qed.
+
+Definition closed_up_to (c:cem.closure) (h:cem.heap) (d:nat) : Prop := match c with
+  | cem.close t e => forevery (fvs' t d) (λ x, ∃ e' c', cem.clu x e h = Some (e',c') ∧ In e' (domain h))
+  end.  
+
+Lemma closed_to_lg : ∀ t e h d, closed_up_to (cem.close t e) h d → ∃ e', 
+  conftolg (cem.conf h (cem.close t e)) d = Some e'.
+intros t. induction t; intros. unfold closed_up_to in H.  rewrite <- gfvs_fvs in
+H. simpl in H. simpl. destruct (gt_dec d n). exists (lvar n).
+reflexivity. simpl in H. destruct H.  destruct H. destruct H. destruct H. 
+rewrite H. simpl. unfold compose.  simpl. exists (gvar x). reflexivity. 
+
+simpl. simpl in H. simpl in IHt. apply IHt in H. destruct H. exists (lam x).
+rewrite H. reflexivity. 
+
+simpl. simpl in H. rewrite forevery_app in H. destruct H. apply IHt1 in H. apply
+IHt2 in H0. destruct H. destruct H0. exists (app x x0). simpl in H. simpl in H0.
+rewrite H. rewrite H0. reflexivity. Qed. 
+
+Lemma wf_to_lg : ∀ c, cem.well_formed c → ∃ e, conftolg c 0 = Some e.
+intros. destruct c. destruct H. unfold cem.closed_under in H. destruct st_clos.
+rewrite fvs_eq_zero in H. apply closed_to_lg in H. assumption. Qed. 
+
+Record configuration := conf {
+  st_heap : Map nat lgexpr;
+  st_clos : lgexpr
+}.
+
+Definition eq_terms (t:expr.tm) (c:cem.configuration) : Prop := 
+  Some (etolg t nil) = conftolg c 0.
+
+Fixpoint related_lists {a b} (la : list a) (lb : list b) (r : a → b → Prop) : Prop :=
+  match la, lb with
+  | x::xs, y::ys => r x y ∧ related_lists xs ys r
+  | nil, nil => True
+  | _, _ => False
+  end.
+
+Definition eq_confs (c: cem.configuration) (c':cbn.configuration) : Prop := 
+  match c, c' with
+  | cem.conf h cl, cbn.st h' e' => eq_terms e' c ∧  related_lists h h' (λ x y, match x,y with
+    | (l, cem.cl c e), (l', t) => eq_terms t (cem.conf h c)
+    end)
+  end.
+
+Lemma expr_closed_under_db: ∀ t xs, expr.fvs t ⊆ domain xs ↔ ∃ e, db t xs = Some e.
+intros t. induction t; intros; split; intros. simpl in H. destruct H. simpl.
+rewrite <- lookup_in_domain_iff in H.  destruct H. rewrite H. exists (db.var x).
+reflexivity. simpl in H. destruct H. remember (lookup n xs). symmetry in Heqo.
+destruct o. apply (ex_intro (λ n0, lookup n xs = Some n0) n0) in Heqo. apply
+lookup_in_domain in Heqo. simpl. split; auto. inversion H. simpl in H. rewrite
+app_subset_and in H. destruct H. apply IHt1 in H. apply IHt2 in H0. destruct H.
+destruct H0. simpl. rewrite H. rewrite H0. exists (db.app x x0). reflexivity.
+simpl in H. simpl. remember (db t1 xs). remember (db t2 xs). destruct o.
+destruct o0. symmetry in Heqo. symmetry in Heqo0. apply (ex_intro (λ x, db t1 xs
+= Some x) t) in Heqo. apply (ex_intro (λ x, db t2 xs = Some x) t0) in Heqo0.
+rewrite <- IHt1 in Heqo. rewrite <- IHt2 in Heqo0. rewrite app_subset_and; 
+split; auto. inversion H. inversion H0. inversion H. inversion H0. simpl in H.
+rewrite <- subset_remove_cons in H. rewrite <- domain_fmap with (f:=S) in H.
+specialize (IHt ((n,0)::map (fmap S) (xs))). simpl in IHt.
+apply IHt in H. simpl. destruct H. rewrite H. exists (db.lam x). reflexivity.
+destruct H. simpl in H. specialize (IHt ((n,0)::map (fmap S) xs)). remember (db
+t ((n,0)::map (fmap S) xs)). destruct o. inversion H. subst. symmetry in Heqo.
+destruct IHt. specialize (H1 (ex_intro (λ e, Some t0 = Some e) t0 eq_refl)).
+simpl. simpl in H1. rewrite domain_fmap in H1. rewrite <- subset_remove_cons.
+assumption. inversion H. Qed. 
+
+Lemma subset_map {A B} : ∀ xs ys (f:A→B), xs ⊆ ys → map f xs ⊆ map f ys. 
+intros xs. induction xs; intros. apply subset_nil. intros. simpl in H. simpl.
+split. destruct H. apply in_map. assumption. apply IHxs. destruct H. assumption.
+Qed. 
+
+Definition homotopy {A B} (f g : A→B) := ∀ x, f x = g x.
+Notation "f ~ g" := (homotopy f g) (at level 60).  
+
+Lemma snd_fmap {A} : (λ x:A*nat, pred (snd (fmap S x))) ~ (λ x:A*nat, snd x). 
+intros. unfold homotopy. intros. destruct x. reflexivity. Qed. 
+
+Lemma map_homo {A B} : ∀ (f g:A→B), f ~ g → map f ~ map g. 
+unfold homotopy. intros. induction x. auto. simpl. rewrite H. rewrite IHx. auto.
+Qed. 
+
+Lemma expr_db_closed : ∀ t e xs, db t xs = Some e → db.fvs e ⊆ codomain xs. 
+intros t. induction t; intros. inversion H. destruct (lookup n xs). inversion
+H1. subst. simpl. split; auto. unfold codomain. inversion H. remember (lookup n
+xs). destruct o. symmetry in Heqo. apply lookup_codomain in Heqo. inversion H2.
+subst. assumption. inversion H2. inversion H1. simpl in H. remember (db t1 xs).
+remember (db t2 xs). destruct o. destruct o0. symmetry in Heqo. symmetry in
+Heqo0. apply IHt1 in Heqo. apply IHt2 in Heqo0. inversion H. subst. simpl.
+rewrite app_subset_and. split; auto. inversion H. inversion H. inversion H.
+remember (db t ((n,0) :: map (fmap S) xs)). destruct o. symmetry in Heqo. apply
+IHt in Heqo. inversion H1. subst. simpl. simpl in Heqo. unfold codomain in Heqo.
+rewrite map_map in Heqo. rewrite subset_remove_cons in Heqo. apply subset_map with
+(f:=pred) in Heqo. rewrite map_map in Heqo. simpl. rewrite (map_homo _ _
+snd_fmap) in Heqo. assumption. inversion H1. Qed. 
+
 
 (*
-Lemma wf_conftolg : ∀ c, cem.well_formed c → ∃ e, conftolg c = Some e.
-intros. destruct c. destruct st_clos. generalize dependent clos_env. generalize
-dependent st_heap. induction clos_tm; intros.  simpl. simpl in H.
-destruct H. destruct H. destruct H. destruct H. destruct H. exists (gvar
-clos_env).  remember (lookup clos_env st_heap). destruct o. destruct c. simpl.
-reflexivity. unfold cem.clu in H. induction n. rewrite <- Heqo in H. inversion
-H.  rewrite <- Heqo in H. inversion H. simpl in H. destruct H.
-remember (db.fvs clos_tm). induction l. assert (map pred (remove 0 nil) = nil).
-reflexivity. rewrite H1 in H. rewrite Heql in H. specialize (IHclos_tm st_heap
-clos_env (conj H H0)). simpl. destruct IHclos_tm. simpl in H2. rewrite H2.   simpl in H. apply IHclos_tm. 
-Definition wf_closure_to_expr : {c | cem.well_formed c} → expr.tm := match 
-
-Definition flatten (c: {c | cem.well_formed c}) : cbn.configuration := match c with
-  | exist (cem.conf h c) p => cbn.st (map (fmap (closure_to_expr ∘ cem.conf h ∘ cem.clclose) h))
-                         (closure_to_expr nil h c)
-  end.
+Lemma eq_initial_confs : ∀ t e, db t nil = Some e → eq_confs 
+  (cem.conf nil (cem.close e 0)) (cbn.st nil t).
+intros. split. unfold eq_terms. unfold conftolg. unfold etolg. induction t; simpl; intros. inversion H. destruct (db t1 nil).
+destruct (db t2 nil). inversion H. subst. split. unfold eq_terms. simpl.
+specialize (IHt1 t eq_refl). simpl in IHt1. unfold eq_terms in IHt1. subst; simpl. simpl in IHt1.
+simpl in IHt2. destruct (2simpl. unfold eq_confs. split. induction t. inversion H. inversion H. simpl. auto. 
 
 (* TODO : Proper relation *)
 Inductive cem_cbn_rel : relation cem.configuration cbn.configuration :=
